proofs/fstar/models/Prost.Error.fsti
@@ -1,6 +1,6 @@
 module Prost.Error
 #set-options "--fuel 0 --ifuel 1 --z3rlimit 15"
-open Core
+open Core_models
 open FStar.Mul
 
 type t_Inner = {
@@ -14,33 +14,33 @@ type t_Inner = {
 /// general it is not possible to exactly pinpoint why data is malformed.
 type t_DecodeError = { f_inner:Alloc.Boxed.t_Box t_Inner Alloc.Alloc.t_Global }
 
-let impl_6: Core.Clone.t_Clone t_DecodeError = { f_clone = (fun x -> x); f_clone_pre = (fun _ -> True); f_clone_post = (fun _ _ -> True) }
+let impl_6: Core_models.Clone.t_Clone t_DecodeError = { f_clone = (fun x -> x); f_clone_pre = (fun _ -> True); f_clone_post = (fun _ _ -> True) }
 
 [@@ FStar.Tactics.Typeclasses.tcinstance]
-val impl_7:Core.Marker.t_StructuralPartialEq t_DecodeError
+val impl_7:Core_models.Marker.t_StructuralPartialEq t_DecodeError
 
 [@@ FStar.Tactics.Typeclasses.tcinstance]
-val impl_8:Core.Cmp.t_PartialEq t_DecodeError t_DecodeError
+val impl_8:Core_models.Cmp.t_PartialEq t_DecodeError t_DecodeError
 
 [@@ FStar.Tactics.Typeclasses.tcinstance]
-val impl_9:Core.Cmp.t_Eq t_DecodeError
+val impl_9:Core_models.Cmp.t_Eq t_DecodeError
 
-let impl_10: Core.Clone.t_Clone t_Inner = { f_clone = (fun x -> x); f_clone_pre = (fun _ -> True); f_clone_post = (fun _ _ -> True) }
-
-[@@ FStar.Tactics.Typeclasses.tcinstance]
-val impl_11:Core.Marker.t_StructuralPartialEq t_Inner
+let impl_10: Core_models.Clone.t_Clone t_Inner = { f_clone = (fun x -> x); f_clone_pre = (fun _ -> True); f_clone_post = (fun _ _ -> True) }
 
 [@@ FStar.Tactics.Typeclasses.tcinstance]
-val impl_12:Core.Cmp.t_PartialEq t_Inner t_Inner
+val impl_11:Core_models.Marker.t_StructuralPartialEq t_Inner
 
 [@@ FStar.Tactics.Typeclasses.tcinstance]
-val impl_13:Core.Cmp.t_Eq t_Inner
+val impl_12:Core_models.Cmp.t_PartialEq t_Inner t_Inner
+
+[@@ FStar.Tactics.Typeclasses.tcinstance]
+val impl_13:Core_models.Cmp.t_Eq t_Inner
 
 /// Creates a new `DecodeError` with a 'best effort' root cause description.
 /// Meant to be used only by `Message` implementations.
 val impl_DecodeError__new
       (#iimpl_270350286_: Type0)
-      {| i1: Core.Convert.t_Into iimpl_270350286_ (Alloc.Borrow.t_Cow string) |}
+      {| i1: Core_models.Convert.t_Into iimpl_270350286_ (Alloc.Borrow.t_Cow string) |}
       (description: iimpl_270350286_)
     : Prims.Pure t_DecodeError Prims.l_True (fun _ -> Prims.l_True)
 
@@ -50,10 +50,10 @@ val impl_DecodeError__push (self: t_DecodeError) (message field: string)
     : Prims.Pure t_DecodeError Prims.l_True (fun _ -> Prims.l_True)
 
 [@@ FStar.Tactics.Typeclasses.tcinstance]
-val impl_1:Core.Fmt.t_Debug t_DecodeError
+val impl_1:Core_models.Fmt.t_Debug t_DecodeError
 
 [@@ FStar.Tactics.Typeclasses.tcinstance]
-val impl_2:Core.Fmt.t_Display t_DecodeError
+val impl_2:Core_models.Fmt.t_Display t_DecodeError
 
 /// A Protobuf message encoding error.
 /// `EncodeError` always indicates that a message failed to encode because the
@@ -64,22 +64,22 @@ type t_EncodeError = {
   f_remaining:usize
 }
 
-let impl_15: Core.Clone.t_Clone t_EncodeError = { f_clone = (fun x -> x); f_clone_pre = (fun _ -> True); f_clone_post = (fun _ _ -> True) }
+let impl_15: Core_models.Clone.t_Clone t_EncodeError = { f_clone = (fun x -> x); f_clone_pre = (fun _ -> True); f_clone_post = (fun _ _ -> True) }
 
 [@@ FStar.Tactics.Typeclasses.tcinstance]
-val impl_14:Core.Marker.t_Copy t_EncodeError
+val impl_14:Core_models.Marker.t_Copy t_EncodeError
 
 [@@ FStar.Tactics.Typeclasses.tcinstance]
-val impl_16:Core.Fmt.t_Debug t_EncodeError
+val impl_16:Core_models.Fmt.t_Debug t_EncodeError
 
 [@@ FStar.Tactics.Typeclasses.tcinstance]
-val impl_17:Core.Marker.t_StructuralPartialEq t_EncodeError
+val impl_17:Core_models.Marker.t_StructuralPartialEq t_EncodeError
 
 [@@ FStar.Tactics.Typeclasses.tcinstance]
-val impl_18:Core.Cmp.t_PartialEq t_EncodeError t_EncodeError
+val impl_18:Core_models.Cmp.t_PartialEq t_EncodeError t_EncodeError
 
 [@@ FStar.Tactics.Typeclasses.tcinstance]
-val impl_19:Core.Cmp.t_Eq t_EncodeError
+val impl_19:Core_models.Cmp.t_Eq t_EncodeError
 
 /// Creates a new `EncodeError`.
 val impl_EncodeError__new (required remaining: usize)
@@ -94,7 +94,7 @@ val impl_EncodeError__remaining (self: t_EncodeError)
     : Prims.Pure usize Prims.l_True (fun _ -> Prims.l_True)
 
 [@@ FStar.Tactics.Typeclasses.tcinstance]
-val impl_4:Core.Fmt.t_Display t_EncodeError
+val impl_4:Core_models.Fmt.t_Display t_EncodeError
 
 /// An error indicating that an unknown enumeration value was encountered.
 /// The Protobuf spec mandates that enumeration value sets are ‘open’, so this
@@ -102,22 +102,22 @@ val impl_4:Core.Fmt.t_Display t_EncodeError
 /// presently used enum definition.
 type t_UnknownEnumValue = | UnknownEnumValue : i32 -> t_UnknownEnumValue
 
-let impl_21: Core.Clone.t_Clone t_UnknownEnumValue = { f_clone = (fun x -> x); f_clone_pre = (fun _ -> True); f_clone_post = (fun _ _ -> True) }
+let impl_21: Core_models.Clone.t_Clone t_UnknownEnumValue = { f_clone = (fun x -> x); f_clone_pre = (fun _ -> True); f_clone_post = (fun _ _ -> True) }
 
 [@@ FStar.Tactics.Typeclasses.tcinstance]
-val impl_20:Core.Marker.t_Copy t_UnknownEnumValue
+val impl_20:Core_models.Marker.t_Copy t_UnknownEnumValue
 
 [@@ FStar.Tactics.Typeclasses.tcinstance]
-val impl_22:Core.Fmt.t_Debug t_UnknownEnumValue
+val impl_22:Core_models.Fmt.t_Debug t_UnknownEnumValue
 
 [@@ FStar.Tactics.Typeclasses.tcinstance]
-val impl_23:Core.Marker.t_StructuralPartialEq t_UnknownEnumValue
+val impl_23:Core_models.Marker.t_StructuralPartialEq t_UnknownEnumValue
 
 [@@ FStar.Tactics.Typeclasses.tcinstance]
-val impl_24:Core.Cmp.t_PartialEq t_UnknownEnumValue t_UnknownEnumValue
+val impl_24:Core_models.Cmp.t_PartialEq t_UnknownEnumValue t_UnknownEnumValue
 
 [@@ FStar.Tactics.Typeclasses.tcinstance]
-val impl_25:Core.Cmp.t_Eq t_UnknownEnumValue
+val impl_25:Core_models.Cmp.t_Eq t_UnknownEnumValue
 
 [@@ FStar.Tactics.Typeclasses.tcinstance]
-val impl_5:Core.Fmt.t_Display t_UnknownEnumValue
+val impl_5:Core_models.Fmt.t_Display t_UnknownEnumValue
