proofs/fstar/models/Num_enum.fsti
@@ -1,6 +1,6 @@
 module Num_enum
 #set-options "--fuel 0 --ifuel 1 --z3rlimit 15"
-open Core
+open Core_models
 open FStar.Mul
 
 (* item error backend: (reject_TraitItemDefault) ExplicitRejection { reason: "a node of kind [Trait_item_default] have been found in the AST" }
@@ -42,8 +42,8 @@ class t_CannotDeriveBothFromPrimitiveAndTryFromPrimitive (v_Self: Type0) = {
 
 (* class t_FromPrimitive (v_Self: Type0) = {
   f_Primitive:Type0;
-  f_Primitive_8876061459599834537:Core.Marker.t_Copy f_Primitive;
-  f_Primitive_17391871992276743015:Core.Cmp.t_Eq f_Primitive;
+  f_Primitive_8876061459599834537:Core_models.Marker.t_Copy f_Primitive;
+  f_Primitive_17391871992276743015:Core_models.Cmp.t_Eq f_Primitive;
   f_from_primitive_pre:f_Primitive -> Type0;
   f_from_primitive_post:f_Primitive -> v_Self -> Type0;
   f_from_primitive:x0: f_Primitive
@@ -52,15 +52,15 @@ class t_CannotDeriveBothFromPrimitiveAndTryFromPrimitive (v_Self: Type0) = {
 
 class t_TryFromPrimitive (v_Self: Type0) = {
   f_Primitive:Type0;
-  (* f_Primitive_12399228673407067350:Core.Marker.t_Copy f_Primitive;
-  f_Primitive_5629480169667985622:Core.Cmp.t_Eq f_Primitive;
-  f_Primitive_10837566226016321784:Core.Fmt.t_Debug f_Primitive; *)
+  (* f_Primitive_12399228673407067350:Core_models.Marker.t_Copy f_Primitive;
+  f_Primitive_5629480169667985622:Core_models.Cmp.t_Eq f_Primitive;
+  f_Primitive_10837566226016321784:Core_models.Fmt.t_Debug f_Primitive; *)
   f_Error:Type0;
   f_NAME:string;
   f_try_from_primitive_pre:f_Primitive -> Type0;
-  f_try_from_primitive_post:f_Primitive -> Core.Result.t_Result v_Self f_Error -> Type0;
+  f_try_from_primitive_post:f_Primitive -> Core_models.Result.t_Result v_Self f_Error -> Type0;
   f_try_from_primitive:x0: f_Primitive
-    -> Prims.Pure (Core.Result.t_Result v_Self f_Error)
+    -> Prims.Pure (Core_models.Result.t_Result v_Self f_Error)
         (f_try_from_primitive_pre x0)
         (fun result -> f_try_from_primitive_post x0 result)
 }
@@ -72,50 +72,50 @@ type t_TryFromPrimitiveError (v_Enum: Type0) (* {| i1: t_TryFromPrimitive v_Enum
 [@@ FStar.Tactics.Typeclasses.tcinstance]
 val impl_5
       (#v_Enum: Type0)
-      {| i1: Core.Clone.t_Clone v_Enum |}
+      {| i1: Core_models.Clone.t_Clone v_Enum |}
       {| i2: t_TryFromPrimitive v_Enum |}
-      {| i3: Core.Clone.t_Clone i2.f_Primitive |}
-    : Core.Clone.t_Clone (t_TryFromPrimitiveError v_Enum)
+      {| i3: Core_models.Clone.t_Clone i2.f_Primitive |}
+    : Core_models.Clone.t_Clone (t_TryFromPrimitiveError v_Enum)
 
 [@@ FStar.Tactics.Typeclasses.tcinstance]
 val impl_4
       (#v_Enum: Type0)
-      {| i1: Core.Marker.t_Copy v_Enum |}
+      {| i1: Core_models.Marker.t_Copy v_Enum |}
       {| i2: t_TryFromPrimitive v_Enum |}
-      {| i3: Core.Marker.t_Copy i2.f_Primitive |}
-    : Core.Marker.t_Copy (t_TryFromPrimitiveError v_Enum)
+      {| i3: Core_models.Marker.t_Copy i2.f_Primitive |}
+    : Core_models.Marker.t_Copy (t_TryFromPrimitiveError v_Enum)
 
 [@@ FStar.Tactics.Typeclasses.tcinstance]
 val impl_6 (#v_Enum: Type0) {| i1: t_TryFromPrimitive v_Enum |}
-    : Core.Marker.t_StructuralPartialEq (t_TryFromPrimitiveError v_Enum)
+    : Core_models.Marker.t_StructuralPartialEq (t_TryFromPrimitiveError v_Enum)
 
 [@@ FStar.Tactics.Typeclasses.tcinstance]
 val impl_7
       (#v_Enum: Type0)
-      {| i1: Core.Cmp.t_PartialEq v_Enum v_Enum |}
+      {| i1: Core_models.Cmp.t_PartialEq v_Enum v_Enum |}
       {| i2: t_TryFromPrimitive v_Enum |}
-      {| i3: Core.Cmp.t_PartialEq i2.f_Primitive i2.f_Primitive |}
-    : Core.Cmp.t_PartialEq (t_TryFromPrimitiveError v_Enum) (t_TryFromPrimitiveError v_Enum)
+      {| i3: Core_models.Cmp.t_PartialEq i2.f_Primitive i2.f_Primitive |}
+    : Core_models.Cmp.t_PartialEq (t_TryFromPrimitiveError v_Enum) (t_TryFromPrimitiveError v_Enum)
 
 [@@ FStar.Tactics.Typeclasses.tcinstance]
 val impl_8
       (#v_Enum: Type0)
-      {| i1: Core.Cmp.t_Eq v_Enum |}
+      {| i1: Core_models.Cmp.t_Eq v_Enum |}
       {| i2: t_TryFromPrimitive v_Enum |}
-      {| i3: Core.Cmp.t_Eq i2.f_Primitive |}
-    : Core.Cmp.t_Eq (t_TryFromPrimitiveError v_Enum)
+      {| i3: Core_models.Cmp.t_Eq i2.f_Primitive |}
+    : Core_models.Cmp.t_Eq (t_TryFromPrimitiveError v_Enum)
 
 val impl__new (#v_Enum: Type0) {| i1: t_TryFromPrimitive v_Enum |} (number: i1.f_Primitive)
     : Prims.Pure (t_TryFromPrimitiveError v_Enum) Prims.l_True (fun _ -> Prims.l_True)
 
 [@@ FStar.Tactics.Typeclasses.tcinstance]
 val impl_1 (#v_Enum: Type0) {| i1: t_TryFromPrimitive v_Enum |}
-    : Core.Fmt.t_Debug (t_TryFromPrimitiveError v_Enum)
+    : Core_models.Fmt.t_Debug (t_TryFromPrimitiveError v_Enum)
 
 [@@ FStar.Tactics.Typeclasses.tcinstance]
 val impl_2 (#v_Enum: Type0) {| i1: t_TryFromPrimitive v_Enum |}
-    : Core.Fmt.t_Display (t_TryFromPrimitiveError v_Enum)
+    : Core_models.Fmt.t_Display (t_TryFromPrimitiveError v_Enum)
 
 [@@ FStar.Tactics.Typeclasses.tcinstance]
 val impl_3 (#v_Enum: Type0) {| i1: t_TryFromPrimitive v_Enum |}
-    : Core.Error.t_Error (t_TryFromPrimitiveError v_Enum)
+    : Core_models.Error.t_Error (t_TryFromPrimitiveError v_Enum)
